snapshot duplicating lemmas; weird error in Associative.lean

src/Std/Data/DHashMap/Basic.lean
@@ -251,12 +251,13 @@ instance [BEq α] [Hashable α] : ForIn m (DHashMap α β) ((a : α) × β a) wh
 Modifies in place the value associated with a given key.
 
 This function ensures that the value is used linearly.
-It is currently implemented in terms of `get?`, `erase`, and `insert`,
-but will later become a primitive operation.
-(It is provided already to help avoid non-linear code.)
 -/
 @[inline] def modify [LawfulBEq α] (m : DHashMap α β) (a : α) (f : β a → β a) : DHashMap α β :=
   ⟨Raw₀.modify (α := α) ⟨m.1, m.2.size_buckets_pos⟩ a f, Raw.WF.modify₀ m.2⟩
+
+@[inline, inherit_doc DHashMap.modify] def Const.modify {β : Type v} (m : DHashMap α (fun _ => β))
+    (a : α) (f : β → β) : DHashMap α (fun _ => β) :=
+  ⟨Raw₀.Const.modify (α := α) ⟨m.1, m.2.size_buckets_pos⟩ a f, Raw.WF.constModify₀ m.2⟩
 
 /--
 Modifies in place the value associated with a given key,
@@ -264,9 +265,13 @@ allowing creating new values and deleting values via an `Option` valued replacem
 
 This function ensures that the value is used linearly.
 -/
-@[inline] def alter {α : Type} {β : α → Type} [BEq α] [Hashable α] [LawfulBEq α] (m : DHashMap α β)
+@[inline] def alter [BEq α] [Hashable α] [LawfulBEq α] (m : DHashMap α β)
     (a : α) (f : Option (β a) → Option (β a)) : DHashMap α β :=
   ⟨Raw₀.alter ⟨m.1, m.2.size_buckets_pos⟩ a f, Raw.WF.alter₀ m.2⟩
+
+@[inline, inherit_doc DHashMap.alter] def Const.alter [BEq α] [Hashable α] {β : Type v}
+    (m : DHashMap α (fun _ => β)) (a : α) (f : Option β → Option β) : DHashMap α (fun _ => β) :=
+  ⟨Raw₀.Const.alter ⟨m.1, m.2.size_buckets_pos⟩ a f, Raw.WF.constAlter₀ m.2⟩
 
 @[inline, inherit_doc Raw.insertMany] def insertMany {ρ : Type w}
     [ForIn Id ρ ((a : α) × β a)] (m : DHashMap α β) (l : ρ) : DHashMap α β :=
