src/Std/Data/DHashMap/Internal/AssocList/Basic.lean
@@ -176,24 +176,51 @@ def modify [BEq α] [LawfulBEq α] (a : α) (f : β a → β a) :
   | cons k v l => if h : k == a then
       have h' : k = a := eq_of_beq h
       let b := f (cast (congrArg β h') v)
-      cons k (cast (congrArg β h'.symm) b) l
+      cons a b l
     else
-      AssocList.cons k v (modify a f l)
+      cons k v (modify a f l)
 
 /-- Internal implementation detail of the hash map -/
 def alter [BEq α] [LawfulBEq α] (a : α) (f : Option (β a) → Option (β a)) :
     AssocList α β → AssocList α β
-  | .nil => match f none with
-    | none => .nil
-    | some b => AssocList.cons a b .nil
-  | .cons k v l => if h : k == a then
+  | nil => match f none with
+    | none => nil
+    | some b => cons a b nil
+  | cons k v l => if h : k == a then
       have h' : k = a := eq_of_beq h
       match f (some (cast (congrArg β h') v)) with
       | none => l
-      | some b => .cons k (cast (congrArg β h'.symm) b) l
+      | some b => cons a b l
     else
       let tail := alter a f l
-      AssocList.cons k v tail
+      cons k v tail
+
+namespace Const
+
+/-- Internal implementation detail of the hash map -/
+def modify [BEq α] {β : Type v} (a : α) (f : β → β) :
+    AssocList α (fun _ => β) → AssocList α (fun _ => β)
+  | nil => nil
+  | cons k v l => if k == a then
+      cons a (f v) l
+    else
+      cons k v (modify a f l)
+
+/-- Internal implementation detail of the hash map -/
+def alter [BEq α] {β : Type v} (a : α) (f : Option β → Option β) :
+    AssocList α (fun _ => β) → AssocList α (fun _ => β)
+  | nil => match f none with
+    | none => nil
+    | some b => AssocList.cons a b nil
+  | cons k v l => if k == a then
+      match f v with
+      | none => l
+      | some b => cons a b l
+    else
+      let tail := alter a f l
+      cons k v tail
+
+end Const
 
 /-- Internal implementation detail of the hash map -/
 @[inline] def filterMap (f : (a : α) → β a → Option (γ a)) :
