src/Std/Data/DHashMap/Internal/AssocList/Lemmas.lean
@@ -241,6 +241,54 @@ theorem modify_eq_alter [BEq α] [LawfulBEq α] {a : α} {f : β a → β a} {l 
   · rfl
   · next ih => simp only [modify, beq_iff_eq, alter, Option.map_some', ih]
 
+namespace Const
+
+variable {β : Type v}
+
+theorem toList_alter [BEq α] [EquivBEq α] {a : α} {f : Option β → Option β} {l : AssocList α (fun _ => β) } :
+    Perm (alter a f l).toList (Const.alterKey a f l.toList) := by
+  rw [Const.alterKey]
+  split
+  · next heq =>
+    induction l
+    · simp only [toList_nil, getValue?_nil] at heq
+      simp only [alter, heq, toList_nil, eraseKey_nil]
+      exact .nil
+    · next ih =>
+      simp only [toList_cons, getValue?_cons, cond_eq_if] at heq
+      split at heq
+      · next heq₂ =>
+        simp only [alter, if_pos heq₂, heq, toList_cons, eraseKey_cons_of_beq heq₂]
+        exact Perm.rfl
+      · next heq₂ =>
+        simp only [alter, if_neg heq₂, toList_cons]
+        simp only [eraseKey_cons_of_false (Bool.not_eq_true _ ▸ heq₂), true_and]
+        exact Perm.cons _ <| ih heq
+  · next heq =>
+    induction l
+    · rw [toList_nil, getValue?_nil] at heq
+      simp only [alter, heq, toList_cons, toList_nil, insertEntry_nil]
+      exact Perm.rfl
+    · next ih =>
+      simp only [toList_cons, getValue?_cons, cond_eq_if] at heq
+      split at heq
+      · next heq₂ =>
+        simp only [alter, heq, if_pos heq₂, toList_cons, insertEntry_cons_of_beq heq₂,
+          List.cons.injEq, and_true]
+        rfl
+      · next heq₂ =>
+        simp only [alter, if_neg heq₂, toList_cons]
+        refine insertEntry_cons_of_false (Bool.not_eq_true _ ▸ heq₂) |>.symm |> Perm.trans ?_
+        exact Perm.cons _ <| ih heq
+
+theorem modify_eq_alter [BEq α] [EquivBEq α] {a : α} {f : β → β} {l : AssocList α (fun _ => β) } :
+    modify a f l = alter a (·.map f) l := by
+  induction l
+  · rfl
+  · next ih => simp only [modify, beq_iff_eq, alter, Option.map_some', ih]
+
+end Const
+
 theorem foldl_apply {l : AssocList α β} {acc : List δ} (f : (a : α) → β a → δ) :
     l.foldl (fun acc k v => f k v :: acc) acc =
       (l.toList.map (fun p => f p.1 p.2)).reverse ++ acc := by
